src/Preamble.v
@@ -1,0 +1,28 @@
+Require Import Coq.Structures.OrderedType.
+Require Import Coq.Structures.OrderedTypeEx.
+Require Import Coq.FSets.FSetAVL.
+Require Import Coq.FSets.FMapAVL.
+Require Coq.FSets.FMapFacts.
+Require Coq.FSets.FSetProperties.
+Require Coq.FSets.FSetBridge.
+
+Module NAME := Nat_as_OT.
+Module NAME_Facts := OrderedTypeFacts NAME.
+Module Set_NAME := FSetAVL.Make NAME.
+Module Set_NAME_Props := FSetProperties.Properties Set_NAME.
+(*Module Set_NAME_Extra := SetUtil Set_NAME.*)
+Module Set_NAME_Dep := FSetBridge.DepOfNodep Set_NAME.
+Module MN := FMapAVL.Make NAME.
+Module MN_Facts := FMapFacts.Facts MN.
+Module MN_Props := FMapFacts.Properties MN.
+(*Module Map_ID_Extra := MapUtil Map_ID.*)
+
+Definition name := NAME.t.
+Definition set_name := Set_NAME.t.
+
+Lemma name_eq_rw:
+  forall k k' : name, k = k' <-> k = k'.
+Proof.
+  intros.
+  auto with *.
+Qed.
