src/Races.v
@@ -1,0 +1,516 @@
+Require Import HJ.Preamble.
+
+Set Implicit Arguments.
+
+Section DoDec.
+  Variable A: Type.
+  Variable P: A -> Prop.
+  Notation Exists:= (exists x, P x).
+  Notation NForall:= (forall x, ~ P x).
+
+  Lemma not_exists_iff:
+    ~ Exists <-> NForall.
+  Proof.
+    intuition.
+    - assert (exists x, P x) by eauto.
+      contradiction.
+    - destruct H0 as (x, H0).
+      eauto.
+  Qed.
+
+  Lemma exists_to_not_nforall:
+    Exists -> ~ NForall.
+  Proof.
+    intros.
+    intuition.
+    destruct H as (x, H).
+    assert (~ P x) by eauto.
+    contradiction.
+  Qed.
+
+  (** In general, it is not possible to conclude the inverse,
+      but if [Exists] is decidable, then we can. *)
+
+  Lemma not_nforall_to_exists:
+     { Exists } + { ~ Exists } ->
+     ~ NForall -> Exists.
+  Proof.
+    intros.
+    destruct H.
+    - assumption.
+    - rewrite not_exists_iff in *.
+      contradiction.
+  Qed.
+
+  Lemma not_forall_iff:
+     { Exists } + { ~ Exists } ->
+     (~ NForall <-> Exists).
+  Proof.
+    intros.
+    split;
+    eauto using exists_to_not_nforall, not_nforall_to_exists.
+  Qed.
+
+  Lemma exists_nforall_dec:
+    { Exists } + { ~ Exists } ->
+    { Exists } + { NForall }.
+  Proof.
+    intros.
+    inversion H.
+    - left; auto.
+    - rewrite not_exists_iff in *.
+      eauto.
+  Qed.
+End DoDec.
+
+Section DoDec2.
+  Variable A: Type.
+  Variable P: A -> Prop.
+  Variable E: Prop.
+  Variable N: Prop.
+
+  Variable exists_alt:
+    E <-> exists x, P x.
+
+  Variable nforall_alt:
+    N <-> (forall x, ~ P x).
+
+  Lemma not_exists_iff_alt:
+    ~ E <-> N.
+  Proof.
+    split;
+    try rewrite exists_alt in *;
+    try rewrite nforall_alt in *;
+    try rewrite not_exists_iff in *;
+    trivial.
+  Qed.
+
+  Lemma exists_to_not_nforall_alt:
+    E -> ~ N.
+  Proof.
+    try rewrite nforall_alt in *;
+    try rewrite exists_alt in *;
+    eauto using exists_to_not_nforall.
+  Qed.
+
+  Let e_to_p:
+    { E } + { ~ E } ->
+    { exists x, P x } + { ~ exists x, P x }.
+  Proof.
+    intros.
+    destruct H; 
+    try rewrite exists_free_alt in *; intuition.
+  Qed.
+
+  Lemma not_nforall_to_exists_alt:
+     { E } + { ~ E } ->
+     ~ N -> E.
+  Proof.
+    intros.
+    apply e_to_p in H.
+    try rewrite exists_alt in *.
+    apply not_nforall_to_exists; auto.
+    intuition.
+  Qed.
+
+  Lemma not_nforall_iff_alt:
+     { E } + { ~ E } ->
+     (~ N <-> E).
+  Proof.
+    intros.
+    split;
+    auto using exists_to_not_nforall_alt, not_nforall_to_exists_alt.
+  Qed.
+
+  Let n_dec_to_e_n:
+    { exists x, P x } + { forall x, ~ P x } ->
+    {E} + {N}.
+  Proof.
+    intros.
+    destruct H.
+    - left; rewrite exists_alt; trivial.
+    - right; rewrite nforall_alt; trivial.
+  Qed.
+
+  Lemma exists_nforall_dec_alt:
+     { E } + { ~ E } ->
+     { E } + { N }.
+  Proof.
+    intros.
+    apply e_to_p in H.
+    apply n_dec_to_e_n.
+    eauto using exists_nforall_dec.
+  Qed.
+
+End DoDec2.
+
+  (** * Races %\&% Dependencies *)
+
+  Inductive tid :=
+  | taskid: name -> tid.
+
+  Definition from_tid t := match t with taskid x => x end.
+
+  Inductive mid :=
+  | memid: name -> mid.
+
+  Definition from_mid t := match t with memid x => x end.
+
+  (** Points-to dependency: a variable points to another variable in the store. *)
+
+  (** Defines a dependency node, that can be either a task name or a memory location. *)
+
+  Notation dep := (mid + tid)%type.
+
+  Notation in_mid := (@inl mid tid).
+
+  Notation in_tid := (@inr mid tid).
+
+  Definition d_mid x := (in_mid (memid x)).
+
+  Definition d_tid x := (in_tid (taskid x)).
+
+  Definition from_dep d := match d with | inl l => from_mid l | inr t => from_tid t end.
+
+Structure DependenciesSpec := {
+  (** Holds when some task is reading from a heap reference. *) 
+
+  Read: tid -> mid -> Prop;
+
+  (** Holds when some task is writing to a heap reference. *)
+
+  Write: tid -> mid -> Prop;
+
+  (** Memory reference points to another reference *)
+
+  PointsTo: mid -> dep -> Prop;
+
+  (**
+    A dependency that goes from a task to a memory location through the
+    local memory of the task. *)
+
+  LocalRef: tid -> mid -> Prop;
+
+
+  (** Blocked dependency: a task is blocked on a future in the taskmap. *)
+
+  Blocked: tid -> tid -> Prop
+}.
+
+Section Defs.
+  Variable D:DependenciesSpec.
+
+  Inductive Race x : Prop :=
+  | race_def:
+    forall t t',
+    Read D t x ->
+    Write D t' x ->
+    Race x.
+
+  Inductive Racy : Prop :=
+  | racy_def:
+    forall x,
+    Race x ->
+    Racy.
+
+  Let racy_alt:
+    Racy <-> exists x, Race x.
+  Proof.
+    split; intros.
+    - inversion H; eauto.
+    - destruct H; eauto using racy_def.
+  Qed.
+
+  Inductive RaceFree : Prop :=
+  | race_free_def:
+    (forall x, ~ Race x) ->
+    RaceFree.
+
+  Let race_free_alt:
+    RaceFree <->
+    (forall x, ~ Race x).
+  Proof.
+    split; intros.
+    - inversion H; eauto.
+    - auto using race_free_def.
+  Qed.
+
+  Lemma not_racy_iff:
+    ~ Racy <-> RaceFree.
+  Proof.
+    apply not_exists_iff_alt with (P:=Race);
+    auto using race_free_alt, racy_alt.
+  Qed.
+
+  Lemma not_race_free_iff:
+     { Racy } + { ~ Racy } ->
+     (~ RaceFree <-> Racy).
+  Proof.
+    apply not_nforall_iff_alt with (P:=Race);
+    auto using race_free_alt, racy_alt.
+  Qed.
+
+  Lemma racy_race_free_dec:
+     { Racy } + { ~ Racy } ->
+     { Racy } + { RaceFree }.
+  Proof.
+    apply exists_nforall_dec_alt with (P:=Race);
+    auto using race_free_alt, racy_alt.
+  Qed.
+
+  (** Dependencies between two names in a state wraps up blocked and points-to
+     dependencies. *)
+
+  Inductive Dep : dep -> dep -> Prop :=
+    | dep_points_to:
+      forall x y,
+      PointsTo D x y ->
+      Dep (inl x) y
+    | dep_blocked:
+      forall x y,
+      Blocked D x y ->
+      Dep (inr x) (inr y)
+    | dep_read:
+      forall x y,
+      Read D x y ->
+      Dep (inr x) (inl y)
+    | dep_reg:
+      forall x y,
+      LocalRef D x y ->
+      Dep (inr x) (inl y).
+
+  (* begin hide *)
+  Require Import Coq.Relations.Relation_Operators.
+  (* end hide *)
+
+  Definition Trans_Blocked := clos_trans _ (Blocked D).
+
+  (** A deadlocked state has a cycle in the [Trans_Blocked] relation. *)
+
+  Inductive Deadlocked : Prop :=
+    deadlocked_def:
+      forall x,
+      Trans_Blocked x x ->
+      Deadlocked.
+
+  Let deadlocked_alt:
+    Deadlocked <-> exists x, Trans_Blocked x x.
+  Proof.
+    split; intros.
+    - inversion H; eauto.
+    - destruct H; eauto using deadlocked_def.
+  Qed.
+
+  Inductive DeadlockFree : Prop :=
+    deadlock_free_def:
+      (forall x, ~ Trans_Blocked x x) ->
+      DeadlockFree.
+
+  Let deadlock_free_alt:
+    DeadlockFree <-> (forall x, ~ Trans_Blocked x x).
+  Proof.
+    split; intros.
+    - inversion H; eauto.
+    - eauto using deadlock_free_def.
+  Qed.
+
+  Lemma not_deadlocked_iff:
+    ~ Deadlocked <-> DeadlockFree.
+  Proof.
+    apply not_exists_iff_alt with (P:=fun x => Trans_Blocked x x);
+    auto using deadlock_free_alt, deadlocked_alt.
+  Qed.
+
+  Lemma not_deadlockfree_iff:
+     { Deadlocked } + { ~ Deadlocked } ->
+     (~ DeadlockFree <-> Deadlocked).
+  Proof.
+    apply not_nforall_iff_alt with (P:=fun x => Trans_Blocked x x);
+    auto using deadlock_free_alt, deadlocked_alt.
+  Qed.
+
+  Lemma deadlocked_deadlockfree_dec:
+     { Deadlocked } + { ~ Deadlocked } ->
+     { Deadlocked } + { DeadlockFree }.
+  Proof.
+    apply exists_nforall_dec_alt with (P:=fun x => Trans_Blocked x x);
+    auto using deadlock_free_alt, deadlocked_alt.
+  Qed.
+
+  (** Defines the [Depends] relation as the transitive closure of [Dep]. *)
+
+  Definition Depends := clos_trans _ Dep.
+
+  (** A state is tainted if there is a cycle in the [Depends] relation.  *) 
+
+  Inductive Tainted : Prop :=
+    tainted_def:
+      forall x,
+      Depends (in_tid x) (in_tid x) ->
+      Tainted.
+
+  Let tainted_alt:
+    Tainted <-> exists x, Depends (in_tid x) (in_tid x).
+  Proof.
+    split; intros.
+    - inversion H; eauto.
+    - destruct H; eauto using tainted_def.
+  Qed.
+
+  Inductive Untainted : Prop :=
+    untainted_def:
+      (forall x, ~ Depends (in_tid x) (in_tid x)) ->
+      Untainted.
+
+  Let untainted_alt:
+    Untainted <-> (forall x, ~ (Depends (in_tid x) (in_tid x))).
+  Proof.
+    split; intros.
+    - inversion H; eauto.
+    - eauto using untainted_def.
+  Qed.
+
+  Let T x := Depends (in_tid x) (in_tid x).
+
+  Lemma not_tainted_iff:
+    ~ Tainted <-> Untainted.
+  Proof.
+    apply not_exists_iff_alt with (P:=T);
+    auto using untainted_alt, tainted_alt.
+  Qed.
+
+  Lemma not_untainted_iff:
+     { Tainted } + { ~ Tainted } ->
+     (~ Untainted <-> Tainted).
+  Proof.
+    apply not_nforall_iff_alt with (P:=T);
+    auto using tainted_alt, untainted_alt.
+  Qed.
+
+  Lemma tainted_untainted_dec:
+     { Tainted } + { ~ Tainted } ->
+     { Tainted } + { Untainted }.
+  Proof.
+    apply exists_nforall_dec_alt with (P:=T);
+    auto using tainted_alt, untainted_alt.
+  Qed.
+
+  Import Operators_Properties.
+
+  Lemma dep_to_depends:
+    forall x y,
+    Dep x y ->
+    Depends x y.
+  Proof.
+    intros.
+    unfold Depends.
+    eauto using t_step.
+  Qed.
+
+  (* XXX: move to Aniceto *)
+  Require Import Coq.Relations.Relation_Definitions.
+
+  Lemma clos_trans_impl:
+    forall {A:Type} (P Q: relation A),
+    (forall x y, P x y -> Q x y) ->
+    forall x y,
+    clos_trans A P x y ->
+    clos_trans A Q x y.
+  Proof.
+    intros.
+    induction H0.
+    - auto using t_step.
+    - eauto using t_trans.
+  Qed.
+
+  Lemma clos_trans_impl_ex:
+    forall {A B:Type} f (P: relation A) (Q: relation B),
+    (forall x y, P x y -> Q (f x) (f y)) ->
+    forall x y,
+    clos_trans A P x y ->
+    clos_trans B Q (f x) (f y).
+  Proof.
+    intros.
+    induction H0.
+    - auto using t_step.
+    - eauto using t_trans.
+  Qed.
+
+  (** A deadlocked state is a special case of a tainted state. *)
+
+  Let trans_blocked_to_depends:
+    forall x,
+    Trans_Blocked x x ->
+    Depends (in_tid x) (in_tid x).
+  Proof.
+    unfold Trans_Blocked, reflexive, Depends in *.
+    eauto using clos_trans_impl_ex, dep_blocked.
+  Qed.
+
+  Lemma deadlocked_to_tainted:
+    Deadlocked ->
+    Tainted.
+  Proof.
+    intros.
+    inversion H.
+    eauto using tainted_def, trans_blocked_to_depends.
+  Qed.
+
+  Lemma untainted_to_deadlockfree:
+    Untainted ->
+    DeadlockFree.
+  Proof.
+    intros.
+    apply not_deadlocked_iff.
+    intuition.
+    apply deadlocked_to_tainted in H0.
+    apply not_tainted_iff in H.
+    contradiction.
+  Qed.
+
+
+(* begin hide *)
+
+End Defs.
+
+Section Props.
+  Lemma deadlocked_impl:
+    forall D E,
+    (forall x y, Blocked D x y -> Blocked E x y) ->
+    Deadlocked D -> Deadlocked E.
+  Proof.
+    intros ? ? Hi Hd.
+    inversion Hd.
+    apply deadlocked_def with (x:=x).
+    unfold Trans_Blocked in *.
+    eauto using clos_trans_impl.
+  Qed.
+
+  Lemma deadlockfree_impl:
+    forall D E,
+    (forall x y, Blocked E x y -> Blocked D x y) ->
+    DeadlockFree D -> DeadlockFree E.
+  Proof.
+    intros ? ? Hi Hd.
+    inversion Hd.
+    apply deadlock_free_def.
+    intros.
+    unfold not; intros.
+    unfold Trans_Blocked in *.
+    assert (Hx := H x).
+    contradiction Hx.
+    eauto using clos_trans_impl.
+  Qed.
+
+End Props.
+
+Section DefsFin.
+  (** Finite definitions of deadlocked and of *)
+  Variable D:DependenciesSpec.
+
+  Inductive DeadlockedOf m : Prop :=
+    deadlock_of:
+      (forall x y, MN.MapsTo x y m <-> Blocked D (taskid x) (taskid y)) ->
+      DeadlockedOf m.
+
+End DefsFin.
